tests/fieldexample.ec
@@ -2,11 +2,12 @@
 require import Int.
 require AlgTactic.
 
+(* -------------------------------------------------------------------- *)
 instance ring with int
   op rzero = Int.zero
   op rone  = Int.one
   op add   = Int.( + )
-  op opp   = [-]
+  op opp   = Int.([-])
   op mul   = Int.( * )
   op expr  = Int.Power.( ^ )
   op sub   = Int.(-)
@@ -24,6 +25,7 @@ instance ring with int
   proof exprS     by smt
   proof subrE     by smt.
 
+(* -------------------------------------------------------------------- *)
 lemma b25  (a b : int):
   (a + b) ^ 25 = ((((((((((((((((((((((((b + 25 * a) * b + 300 * a ^ 2) * b + 2300 * a ^ 3) *
                      b + 12650 * a ^ 4) *
@@ -53,35 +55,66 @@ proof. by ring. qed.
 lemma binom (x y : int): (x+y)^2 = x^2 + 2 * x * y + y^2.
 proof. by ring. qed.
 
-(*
-require import Prime_field.
+(* -------------------------------------------------------------------- *)
+require Prime_field.
 
 const k : int.
 
-axiom k_pos : 0 <= k.
+axiom ge0_k : 0 <= k.
 
 clone import Prime_field as Zq with op q = k.
 
 type zq = Zq.gf_q.
 
-op uint : zq distr = Zq.Dgf_q.dgf_q.
+op (^^) : zq -> int -> zq.
 
-import Zq.
+axiom qf_expr0 : forall (x : zq), x^^0 = gf_q1.
+axiom qf_exprS : forall (x : zq) i, 0 <= i => x^^(i+1) = x * x^^i.
+axiom qf_exprN : forall (x : zq) i, 0 <= i => x^^(-i) = inv (x^^i).
 
-op ( ^^ ) : zq -> int -> zq.
-axiom pow1 : forall (a : zq), forall ( i : int), i > 0 => a ^^ i = Zq.( * ) a (a ^^ (i-1)).
-axiom pow0 : forall (a : zq), a <> Zq.gf_q0 =>  a ^^ 0 = Zq.gf_q1.
-axiom pow00 : forall ( i : int), Zq.gf_q0 ^^ i = Zq.gf_q0.
+op ofint : int -> zq.
 
-lemma rbinom : forall (x y : zq),
-    Zq.( * ) ((Zq.(-) x y) ^^ 2 ) (Zq.(+) Zq.gf_q1 Zq.gf_q1) = 
-    Zq.( * ) ( Zq.(-) (Zq.(+) ( x ^^ 2) (y ^^ 2)) ( Zq.( * ) (Zq.(+) x x) y)) (Zq.(+) Zq.gf_q1 Zq.gf_q1).
-proof.
-intros x y.
-(*ring Zq.(+) Zq.( * ) ( ^^ ) Zq.(-) Zq.gf_q0 Zq.gf_q1 ( = ).*)
-field Zq.(+) Zq.( * ) ( ^^ ) Zq.inv Zq.(-) Zq.(/) Zq.gf_q0 Zq.gf_q1 (=).
-qed.
+axiom qf_ofint0 : ofint 0 = Zq.gf_q0.
+axiom qf_ofint1 : ofint 1 = Zq.gf_q1.
+axiom qf_ofintS : forall i, 0 <= i => ofint (i+1) = ofint i + gf_q1.
+axiom qf_ofintN : forall (i : int), ofint (-i) = -(ofint i).
 
+instance field with zq
+  op rzero = Zq.gf_q0
+  op rone  = Zq.gf_q1
+  op add   = Zq.( + )
+  op opp   = Zq.([-])
+  op mul   = Zq.( * )
+  op expr  = (^^)
+  op sub   = Zq.( - )
+  op ofint = ofint
+  op inv   = Zq.inv
+  op div   = Zq.(/)
+
+  proof oner_neq0 by smt
+  proof addr0     by smt
+  proof addrA     by smt
+  proof addrC     by smt
+  proof addrN     by smt
+  proof mulr1     by smt
+  proof mulrA     by smt
+  proof mulrC     by smt
+  proof mulrDl    by smt
+  proof mulrV     by smt
+  proof expr0     by smt
+  proof exprS     by smt
+  proof exprN     by smt
+  proof subrE     by smt
+  proof divrE     by smt
+  proof ofint0    by smt
+  proof ofint1    by smt
+  proof ofintS    by smt
+  proof ofintN    by smt.
+
+lemma rbinom (x y : zq): (x - y)^^2 = x^^2 - (ofint 2) * x * y + y^^2.
+proof. by field. qed.
+
+(* FIXME: to be sync'ed with new ring/field tactics
 lemma b24 : forall (a b c: zq) ,
     a = b =>
     c = (Zq.( * ) (Zq.(+) Zq.gf_q1 Zq.gf_q1) a) =>
@@ -100,40 +133,6 @@ intros a b c T U.
 field Zq.(+) Zq.( * ) ( ^^ ) Zq.inv Zq.(-) Zq.(/) Zq.gf_q0 Zq.gf_q1 (=) T U.
 qed.
 
-lemma b25 : forall (a b : int) , (a + b) ^ 25 = ((((((((((((((((((((((((b + 25 * a) * b + 300 * a ^ 2) * b + 2300 * a ^ 3) *
-                     b + 12650 * a ^ 4) *
-                    b + 53130 * a ^ 5) *
-                   b + 177100 * a ^ 6) *
-                  b + 480700 * a ^ 7) *
-                 b + 1081575 * a ^ 8) *
-                b + 2042975 * a ^ 9) *
-               b + 3268760 * a ^ 10) *
-              b + 4457400 * a ^ 11) *
-             b + 5200300 * a ^ 12) *
-            b + 5200300 * a ^ 13) *
-           b + 4457400 * a ^ 14) *
-          b + 3268760 * a ^ 15) *
-         b + 2042975 * a ^ 16) *
-        b + 1081575 * a ^ 17) *
-       b + 480700 * a ^ 18) *
-      b + 177100 * a ^ 19) *
-     b + 53130 * a ^ 20) *
-    b + 12650 * a ^ 21) *
-   b + 2300 * a ^ 22) *
-  b + 300 * a ^ 23) *
- b + 25 * a ^ 24) *
-b + (a ^ 25).
-proof.
-intros a b.
-ring Int.(+) Int.( * ) (^) Int.(-) 0 1 ( = ).
-qed.
-
-lemma binom : forall (x y : int), ((x+y) ^2) = (x^2 + 2* x * y + y^2).
-proof.
-intros x y.
-ring Int.(+) Int.( * ) (^) Int.(-) 0 1 ( = ).
-(*field (+) ( * ) ( ^ ) inv (-) (/) 0 1 (=).*)
-qed.
 
 (* OT examples*)
 
